theories/Misc/Pure.v
@@ -3,11 +3,14 @@ From CTree Require Import
 
 Variant pureb {E C X} (rec : ctree E C X -> Prop) (t : ctree E C X) : Prop :=
   | pureb_ret   (v : X) (EQ : t ≅ Ret v) : pureb rec t
-  | pureb_delay {Y} (c: C Y) k (EQ : t ≅ BrD c k) (REC: forall v, rec (k v)) : pureb rec t.
+  | pureb_stuck (EQ : t ≅ Stuck) : pureb rec t
+  | pureb_br {Y} (c: C Y) k (EQ : t ≅ Br c k) (REC: forall v, rec (k v)) : pureb rec t
+  | pureb_guard  u (EQ : t ≅ Guard u) (REC: rec u) : pureb rec t.
+Hint Constructors pureb: core.
 
 Program Definition fpure {E C R} : mon (ctree E C R -> Prop) := {|body := pureb|}.
 Next Obligation.
-  inversion_clear H0; [eleft | eright]; eauto.
+  inversion_clear H0; eauto.
 Qed.
 
 Section pure.
@@ -18,49 +21,57 @@ Section pure.
 
   #[global] Instance pure_equ : Proper (@equ E C X X eq ==> flip impl) pure.
   Proof.
-    cbn. intros. step in H0. inversion H0.
-    - step. eleft. now rewrite H, EQ.
-    - step. eright. now rewrite H, EQ. apply REC.
+    cbn. intros. step in H0. inversion H0; step;
+      [econstructor 1 | econstructor 2 | econstructor 3 | econstructor 4]; eauto.
+    all: rewrite H, EQ; eauto.
   Qed.
 
   #[global] Instance pure_ret r : pure (Ret r).
   Proof.
-    step. now eleft.
+    step; cbn; eauto.
   Qed.
 
   #[global] Instance pure_br {T} (c : C T) k :
     (forall x, pure (k x)) ->
-    pure (BrD c k).
+    pure (Br c k).
   Proof.
-    intros. step. now eright.
+    intros; step; cbn; eauto.
   Qed.
 
-  #[global] Instance pure_guard `{B1 -< C} t :
+  #[global] Instance pure_guard t :
     pure t ->
     pure (Guard t).
   Proof.
-    intros. unfold Guard. step. now eright.
+    intros; step; cbn; eauto.
   Qed.
 
-  #[global] Instance pure_stuck `{B0 -< C} :
-    pure stuckD.
+  #[global] Instance pure_stuck :
+    pure Stuck.
   Proof.
-    unfold stuckD. step. now eright.
+    intros; step; cbn; eauto.
   Qed.
 
-  Lemma pure_brD_inv : forall {X} (c : C X) k x,
-    pure (BrD c k) ->
+  Lemma pure_br_inv : forall {X} (c : C X) k x,
+    pure (Br c k) ->
     pure (k x).
   Proof.
     intros. step in H. inv H; inv_equ.
     rewrite EQ0. apply REC.
   Qed.
 
+  Lemma pure_guard_inv : forall t,
+    pure (Guard t) ->
+    pure t.
+  Proof.
+    intros. step in H. inv H; inv_equ.
+    rewrite EQ. apply REC.
+  Qed.
+
   Lemma pure_productive : forall (t : ctree E C X),
     pure t -> productive t -> exists r, t ≅ Ret r.
   Proof.
     intros. step in H. inv H; eauto.
-    rewrite EQ in H0. inv H0; inv_equ.
+    all: rewrite EQ in H0; inv H0; inv_equ.
   Qed.
 
   Lemma pure_epsilon :
@@ -69,36 +80,55 @@ Section pure.
     intros. rewrite ctree_eta in H. rewrite ctree_eta. red in H0. genobs t ot. genobs t' ot'.
     clear t t' Heqot Heqot'. induction H0.
     - now subs.
-    - apply IHepsilon_. rewrite <- ctree_eta. eapply pure_brD_inv. apply H.
+    - apply IHepsilon_. rewrite <- ctree_eta. eapply pure_br_inv. apply H.
+    - apply IHepsilon_. rewrite <- ctree_eta. eapply pure_guard_inv. apply H.
   Qed.
 
-  Lemma trans_pure_is_val `{B0 -< C} (t t' : ctree E C X) l :
+  Lemma trans_pure_is_val (t t' : ctree E C X) l :
     pure t ->
     trans l t t' ->
     is_val l.
   Proof.
-    intros. do 3 red in H1. genobs t ot. genobs t' ot'.
+    intros. do 3 red in H0. genobs t ot. genobs t' ot'.
     assert (t ≅ go ot). { now rewrite Heqot, <- ctree_eta. } clear Heqot.
-    revert t H0 H2. induction H1; intros; subst.
+    revert t H H1. induction H0; intros; subst.
     - apply IHtrans_ with (t := k x); auto. 2: apply ctree_eta.
-      rewrite H2 in H0. step in H0. inversion H0; inv_equ.
+      rewrite H1 in H. step in H. inversion H; inv_equ.
       rewrite EQ0. apply REC.
-    - rewrite H2 in H1. step in H1. inversion H1; inv_equ.
-    - rewrite H2 in H1. step in H1. inversion H1; inv_equ.
+    - apply IHtrans_ with t; eauto. 2: apply ctree_eta.
+      rewrite H1 in H; step in H; inversion H; inv_equ.
+      rewrite EQ. apply REC.
+    - rewrite H1 in H0. step in H0. inversion H0; inv_equ.
+    - rewrite H1 in H0. step in H0. inversion H0; inv_equ.
     - constructor.
   Qed.
 
-  Lemma trans_bind_pure {Y} `{B0 -< C} (t : ctree E C X) k (u : ctree E C Y) l :
+  Lemma trans_bind_pure {Y} (t : ctree E C X) k (u : ctree E C Y) l :
     pure t ->
     trans l (CTree.bind t k) u ->
-    exists v, trans (val v) t stuckD /\ trans l (k v) u.
+    exists v, trans (val v) t Stuck /\ trans l (k v) u.
   Proof.
-    intros. apply trans_bind_inv in H1 as [(? & ? & ? & ?) |].
-    - now apply trans_pure_is_val in H2.
-    - apply H1.
+    intros. apply trans_bind_inv in H0 as [(? & ? & ? & ?) |].
+    - now apply trans_pure_is_val in H1.
+    - apply H0.
   Qed.
 
 End pure.
+
+(* TO MOVE *)
+Lemma map_stuck {E B X Y} (f : X -> Y) :
+    @CTree.map E B _ _ f Stuck ≅ Stuck.
+Proof.
+  intros. unfold CTree.map.
+  apply bind_stuck.
+Qed.
+
+Lemma map_br {E B X Y Z} (e : B Z) k (f : X -> Y) :
+    @CTree.map E B _ _ f (Br e k) ≅ Br e (fun x => CTree.map f (k x)).
+Proof.
+  intros. unfold CTree.map.
+  apply bind_br.
+Qed.
 
 #[global] Instance pure_map {E B X Y} : forall (t : ctree E B X) (f : X -> Y),
   pure t ->
@@ -106,10 +136,10 @@ End pure.
 Proof.
   red. coinduction R CH. intros.
   step in H. destruct H.
-  - eleft. rewrite EQ. rewrite map_ret. reflexivity.
-  - eright.
-    + rewrite EQ. unfold CTree.map. rewrite bind_br. reflexivity.
-    + intros. apply CH. apply REC.
+  - econstructor 1; rewrite EQ, map_ret; reflexivity.
+  - econstructor 2. rewrite EQ, map_stuck; reflexivity.
+  - econstructor 3. rewrite EQ, map_br; reflexivity. intros; apply CH, REC.
+  - econstructor 4. rewrite EQ, map_guard; reflexivity. intros; apply CH, REC.
 Qed.
 
 Section pure_finite.
@@ -117,8 +147,10 @@ Section pure_finite.
   Context {E C : Type -> Type} {X : Type}.
 
   Inductive pure_finite_ : ctree E C X -> Prop :=
-    | puref_ret (v : X) t (EQ: t ≅ Ret v) : pure_finite_ t
-    | puref_delay {Y} (c: C Y) (k : Y -> ctree E C X) t (EQ: t ≅ BrD c k) (REC: forall v, pure_finite_ (k v)) : pure_finite_ t.
+  | puref_ret (v : X) t (EQ: t ≅ Ret v) : pure_finite_ t
+  | puref_stuck t (EQ : t ≅ Stuck) : pure_finite_ t
+  | puref_br {Y} (c: C Y) k t (EQ : t ≅ Br c k) (REC: forall v, pure_finite_ (k v)) : pure_finite_ t
+  | puref_guard t u (EQ : t ≅ Guard u) (REC: pure_finite_ u) : pure_finite_ t.
 
   Class pure_finite (t : ctree E C X) : Prop :=
     pure_finite__ : pure_finite_ t.
@@ -127,34 +159,34 @@ Section pure_finite.
     Proper (equ eq ==> flip impl) pure_finite.
   Proof.
     cbn. intros. revert x H. induction H0; intros.
-    - eleft. now subs.
-    - eright. now subs.
-      intro. now eapply H.
+    - econstructor 1; now subs.
+    - econstructor 2; now subs.
+    - econstructor 3; now subs.
+    - econstructor 4; now subs.
   Qed.
 
   #[global] Instance pure_finite_ret r : pure_finite (Ret r).
   Proof.
-    now eleft.
+    now econstructor 1.
+  Qed.
+
+  #[global] Instance pure_finite_stuck : pure_finite Stuck.
+  Proof.
+    now econstructor 2.
   Qed.
 
   #[global] Instance pure_finite_br {T} (c : C T) k :
     (forall x, pure_finite (k x)) ->
-    pure_finite (BrD c k).
+    pure_finite (Br c k).
   Proof.
-    now eright.
+    now econstructor 3.
   Qed.
 
-  #[global] Instance pure_finite_guard `{B1 -< C} t :
+  #[global] Instance pure_finite_guard t :
     pure_finite t ->
     pure_finite (Guard t).
   Proof.
-    unfold Guard. now eright.
-  Qed.
-
-  #[global] Instance pure_finite_stuck `{B0 -< C} :
-    pure_finite stuckD.
-  Proof.
-    unfold stuckD. now eright.
+    now econstructor 4.
   Qed.
 
 End pure_finite.
@@ -168,7 +200,9 @@ Lemma pure_finite_bind_R {E C X Y} :
 Proof.
   intros. induction H0.
   - subs. inv_equ. rewrite bind_ret_l; auto.
+  - subs. rewrite bind_stuck. apply pure_finite_stuck.
   - subs. inv_equ. rewrite bind_br. apply pure_finite_br. auto.
+  - subs. inv_equ. rewrite bind_guard. apply pure_finite_guard. auto.
 Qed.
 
 #[global] Instance pure_finite_bind {E C X Y} :
@@ -186,20 +220,22 @@ Qed.
   pure t.
 Proof.
   intros. induction H; subs; step.
-  - now eleft.
-  - now eright.
-Qed.
+    - econstructor 1; now subs.
+    - econstructor 2; now subs.
+    - econstructor 3; now subs.
+    - econstructor 4; now subs.
+  Qed.
 
-Lemma is_stuck_pure : forall {E B X Y} `{B0 -< B} t (k : X -> ctree E B Y),
+Lemma is_stuck_pure : forall {E B X Y} t (k : X -> ctree E B Y),
   pure t ->
   (forall x, is_stuck (k x)) ->
   is_stuck (CTree.bind t k).
 Proof.
   red. intros. intro.
-  apply trans_bind_inv in H2 as [].
-  - destruct H2 as (? & ? & ? & ?). subs.
-    apply H2. eapply trans_pure_is_val; eauto.
-  - destruct H2 as (? & ? & ?). now apply H1 in H3.
+  apply trans_bind_inv in H1 as [].
+  - destruct H1 as (? & ? & ? & ?). subs.
+    apply H1. eapply trans_pure_is_val; eauto.
+  - destruct H1 as (? & ? & ?). now apply H0 in H2.
 Qed.
 
 (*|
@@ -207,10 +243,9 @@ A computation [is_simple] all its transitions are either:
 - directly returning
 - or reducing in one step to something of the shape [Guard* (Ret r)]
 |*)
-Class is_simple {E C X} (t : ctree E (B01 +' C) X) :=
+Class is_simple {E C X} (t : ctree E C X) :=
   is_simple' : (forall l t', trans l t t' -> is_val l) \/
   (forall l t', trans l t t' -> exists r, epsilon_det t' (Ret r)).
-
 
 Section is_simple_theory.
 
@@ -222,26 +257,26 @@ Section is_simple_theory.
     cbn. intros. unfold is_simple. setoid_rewrite H. reflexivity.
   Qed.
 
-  #[global] Instance is_simple_ret : forall r, is_simple (Ret r : ctree E (B01 +' C) X).
+  #[global] Instance is_simple_ret : forall r, is_simple (Ret r : ctree E C X).
   Proof.
     cbn. red. intros. left. intros. inv_trans. subst. constructor.
   Qed.
 
   #[global] Instance is_simple_guard_ret : forall r,
-      is_simple (Guard (Ret r) : ctree E (B01 +' C) X).
+      is_simple (Guard (Ret r) : ctree E C X).
   Proof.
     cbn. red. intros. left. intros. inv_trans. subst. constructor.
   Qed.
 
-  #[global] Instance is_simple_br : forall (c: (B01 +' C) X),
-      is_simple (branchD c : ctree E (B01 +' C) X).
+  #[global] Instance is_simple_br : forall (c: C X),
+      is_simple (CTree.branch c : ctree E C X).
   Proof.
     cbn. red. intros.
-    left. intros. apply trans_brD_inv in H as []. inv_trans. subst. constructor.
+    left. intros. apply trans_br_inv in H as []. inv_trans. subst. constructor.
   Qed.
 
   #[global] Instance is_simple_map :
-    forall {Y} (t : ctree E (B01 +' C) X) (f : X -> Y),
+    forall {Y} (t : ctree E C X) (f : X -> Y),
     is_simple t -> is_simple (CTree.map f t).
   Proof.
     intros. destruct H.
@@ -259,7 +294,7 @@ Section is_simple_theory.
   Qed.
 
   #[global] Instance is_simple_liftState {St} :
-    forall (t : ctree E (B01 +' C) X) (s : St),
+    forall (t : ctree E C X) (s : St),
     is_simple t -> is_simple (Monads.liftState t s).
   Proof.
     intros. cbn. typeclasses eauto.
@@ -267,15 +302,15 @@ Section is_simple_theory.
 
   #[global] Instance is_simple_trigger :
     forall (e : E X),
-    is_simple (CTree.trigger e : ctree E (B01 +' C) X).
+    is_simple (CTree.trigger e : ctree E C X).
   Proof.
     right. intros.
     unfold CTree.trigger in H. inv_trans. subst.
     exists x. now left.
   Qed.
 
-  Lemma is_simple_brD_inv : forall {Y} (c: (B01 +' C) X) (k : X -> ctree E (B01 +' C) Y) x,
-      is_simple (BrD c k) -> is_simple (k x).
+  Lemma is_simple_br_inv : forall {Y} (c: C X) (k : X -> ctree E C Y) x,
+      is_simple (Br c k) -> is_simple (k x).
   Proof.
     intros. destruct H.
     - left. intros. eapply H. etrans.
@@ -283,7 +318,7 @@ Section is_simple_theory.
   Qed.
 
   #[global] Instance is_simple_pure :
-    forall (t : ctree E (B01 +' C) X),
+    forall (t : ctree E C X),
     pure t -> is_simple t.
   Proof.
     left. intros. eapply trans_pure_is_val; eassumption.
